matching-logic/src/Utils/extralibrary.v
@@ -293,3 +293,23 @@ Tactic Notation "destruct_and" "?" :=
   repeat match goal with H : _ |- _ => progress (destruct_and? H) end.
 Tactic Notation "destruct_and" "!" :=
   progress destruct_and?.
+
+
+Tactic Notation "destruct_or" "?" ident(H) :=
+  repeat
+    (match type of H with
+     | is_true false => inversion H
+     | False => destruct H
+     | _ ∨ _ => destruct H as [H|H]
+     | Is_true (bool_decide _) => apply (bool_decide_unpack _) in H
+     | Is_true (_ || _) => apply orb_True in H; destruct H as [H|H]
+     | is_true (_ || _) => apply orb_true_iff in H; destruct H as [H|H]
+     | (_ || _) = true => apply orb_true_iff in H; destruct H as [H|H]
+     end).
+
+Tactic Notation "destruct_or" "!" ident(H) := hnf in H; progress (destruct_or? H).
+
+Tactic Notation "destruct_or" "?" :=
+  repeat match goal with H : _ |- _ => progress (destruct_or? H) end.
+Tactic Notation "destruct_or" "!" :=
+  progress destruct_or?.
